src/tree/layer1/OrderedSetUtils.dfy
@@ -1,0 +1,297 @@
+
+
+function isSortedSeq(xs:seq<int>):bool
+{forall i,j::0<=i<j<|xs| ==> xs[i]<xs[j]}
+
+function Pick(s: set<int>): int
+  requires s != {}
+{
+  var x :| x in s; x
+}
+
+function seq2Set (xs:seq<int>):set<int>
+{set x | x in xs::x}
+
+function set2Seq(s:set<int>):seq<int>
+decreases s
+{
+  if s == {} then []
+  else 
+    var y := Pick(s);
+    [y] + set2Seq(s - {y})
+    
+}
+
+lemma sizesSet2Seq(s:set<int>)
+ensures |set2Seq(s)|==|s|
+{}
+
+lemma  sizesSeq2Set(xs:seq<int>)
+requires forall i,j|0 <= i < j < |xs| :: xs[i] != xs[j]
+ensures |seq2Set(xs)| == |xs|
+{if (xs==[]) {}
+ else {sizesSeq2Set(xs[1..]);
+       assert xs==[xs[0]]+xs[1..];
+       assert seq2Set(xs)=={xs[0]}+seq2Set(xs[1..]);
+       assert |seq2Set(xs)|==1+|seq2Set(xs[1..])|;}
+}
+
+lemma idem(s:set<int>)
+ensures seq2Set(set2Seq(s)) == s 
+{  if s != {} {
+    var y := Pick(s);
+    assert seq2Set([y] + set2Seq(s - {y})) == seq2Set([y]) + seq2Set(set2Seq(s - {y}));
+  }
+}
+
+function sort(xs:seq<int>):seq<int>
+ensures seq2Set(xs)==seq2Set(sort(xs)) && isSortedSeq(sort(xs))
+ensures |xs|==|sort(xs)|
+
+function set2SortedSeq(s:set<int>):seq<int>
+ensures set2SortedSeq(s)==sort(set2Seq(s))
+{sort(set2Seq(s))
+}
+
+lemma sortedSeq(s:set<int>)
+ensures isSortedSeq(set2SortedSeq(s)) && seq2Set(set2SortedSeq(s))==s
+ensures |set2SortedSeq(s)|==|s|
+{idem(s);sizesSet2Seq(s);}
+
+
+lemma sizeOfSet(s:set<int>,x:int)
+requires x in s
+ensures (s-{x})+{x}==s
+{}
+
+lemma sizes(s1:set<int>,s2:set<int>)
+requires s1==s2
+ensures |s1|==|s2|
+{}
+//MINIMUM DEFINITION:  
+
+function {:induction s} minimum(s:set<int>):int
+requires s != {}
+//ensures forall x | x in s :: minimum(s)<=x
+{ 
+  var x :| x in s;
+  if (s-{x}=={}) then x
+  else if (x < minimum(s-{x})) then x
+  else minimum(s-{x})
+
+}
+
+// Minimum is smaller or equal than all the set elements
+lemma lmin(s:set<int>,x:int)
+requires s!={} && x in s
+ensures x>=minimum(s)
+{
+  var y:| y in s;
+  if (s-{y} == {}){assert s=={y};assert x==y;}
+  else if (minimum(s-{y})==minimum(s)){}
+  else{}
+}
+
+
+lemma lminimum(s:set<int>)
+requires s != {}
+ensures minimum(s) in s && forall x | x in s :: minimum(s) <= x
+{forall x | x in s
+ ensures minimum(s) <= x {lmin(s,x);}}
+
+//An element smaller than the rest of elements is the minimum
+lemma lminimumrev(s:set<int>,x:int)
+requires x in s && forall z | z in s && z!=x :: x < z
+ensures x == minimum(s)
+{
+  lminimum(s);
+   assert minimum(s) in s;
+   if (x==minimum(s)){}
+   else {assert x < minimum(s);
+         assert false;}//contradiction
+}
+
+//MAXIMUM DEFINITION: 
+function {:induction s} maximum(s:set<int>):int
+requires s != {}
+{ 
+  var x :| x in s;
+  if (s-{x}=={}) then x
+  else if (x > maximum(s-{x})) then x
+  else maximum(s-{x})
+  
+}
+
+//Maximum is bigger or equal than all the set elements 
+lemma lmax(s:set<int>,x:int)
+requires s!={} && x in s
+ensures x<=maximum(s)
+{
+  var y:| y in s;
+  if (s-{y} == {}){assert s=={y};assert x==y;}
+  else if (maximum(s-{y})==maximum(s)){}
+  else{}
+}
+
+
+//maximum belongs to the set
+lemma lmaximum(s:set<int>)
+requires s != {}
+ensures maximum(s) in s && forall x | x in s :: maximum(s) >= x
+ensures forall x | x in s && s-{x}!={} && x > maximum(s-{x}) :: x==maximum(s) 
+ensures forall x | x in s && s-{x}!={} && x <= maximum(s-{x}) :: maximum(s)==maximum(s-{x}) 
+{forall x | x in s
+ ensures maximum(s) >= x {lmax(s,x);}}
+
+lemma lmaximumOne(s:set<int>,x:int)
+requires s!={} && x in s && s-{x}!={} 
+ensures if (x <= maximum(s-{x})) then maximum(s) == maximum(s-{x}) else maximum(s)==x
+{
+  lmaximum(s);
+}
+
+//Any element of the set bigger tahn the rest is the maximum
+lemma lmaximumrev(s:set<int>,x:int)
+requires x in s && forall z | z in s && z!=x :: x > z
+ensures x == maximum(s)
+{
+  lmaximum(s);
+   assert maximum(s) in s;
+   if (x==maximum(s)){}
+   else {assert x > maximum(s);
+         assert false;}//contradiction
+}
+
+lemma lmaximum2(s:set<int>,x:int)
+requires s!={} && x in s && s-{x}!={} && x < maximum(s-{x})
+ensures maximum(s)!=x 
+{lmaximum(s-{x});
+assert maximum(s-{x}) in s;
+lmax(s,maximum(s-{x}));
+assert maximum(s-{x})<= maximum(s);
+assert exists z | z in s :: z < maximum(s);
+}
+
+
+//If the set has two elements, if I remove the minimun, the maximum is the same: needed to prove First and Last
+lemma max2Elems(s:set<int>)
+requires |s|>=2
+ensures s-{minimum(s)} != {} && maximum(s)==maximum(s-{minimum(s)})
+{
+  lminimum(s);
+  assert |s-{minimum(s)}|==|s|-1>=1;
+  //assert s-{minimum(s)} != {};
+  lmax(s,minimum(s));
+  assert minimum(s) in s && minimum(s) < maximum(s-{minimum(s)});
+  lmaximumOne(s,minimum(s)); 
+
+}
+
+lemma {:verify true} lMaxMinOne(s:set<int>)
+requires s != {} && |s|==1
+ensures maximum(s)==minimum(s)
+{}
+
+function smaller(s:set<int>,x:int):set<int>
+ensures forall z | z in smaller(s,x) :: z in s && z < x
+ensures forall z | z in s && z < x :: z in smaller(s,x)
+{set z | z in s && z < x}
+
+
+
+lemma {:verify true} smallerMin(s:set<int>)
+requires s != {}
+ensures smaller(s,minimum(s))=={} && |smaller(s,minimum(s))|==0
+{}
+
+
+lemma {:verify true} smallerMax(s:set<int>)
+requires s != {}
+ensures smaller(s,maximum(s))==s-{maximum(s)} && |smaller(s,maximum(s))|== |s|-1
+{ sizes(smaller(s,maximum(s)),s-{maximum(s)});
+  assert |smaller(s,maximum(s))|==|s-{maximum(s)}|;
+  lmaximum(s);
+  sizeOfSet(s,maximum(s));
+  }
+  
+
+function elemth(s:set<int>,k:int):int
+requires 0<=k<|s|
+//ensures elemth(s,k) in s && |smaller(s,elemth(s,k))|==k
+{
+  var minim:=minimum(s);
+  if (k==0) then minim
+  else elemth(s-{minim},k-1)
+}
+
+lemma {:induction s,k} {:verify true} lelemth(s:set<int>,k:int)
+requires 0<=k<|s|
+ensures elemth(s,k) in s && |smaller(s,elemth(s,k))|==k
+{ lminimum(s);
+  if (k==0) { }
+  else {
+    lelemth(s-{minimum(s)},k-1);
+    assert elemth(s,k) in s;
+    calc =={
+      |smaller(s,elemth(s,k))|;
+      |set z | z in s && z < elemth(s,k)|;{assert k>0;}
+      |set z | z in s && z < elemth(s-{minimum(s)},k-1)|;
+      {assert s==(s-{minimum(s)})+{minimum(s)};
+      assert minimum(s)<elemth(s-{minimum(s)},k-1);
+      assert (set z | z in s && z < elemth(s-{minimum(s)},k-1))==(set z | z in s-{minimum(s)} && z < elemth(s-{minimum(s)},k-1)) + {minimum(s)};
+      }
+      |(set z | z in s-{minimum(s)} && z < elemth(s-{minimum(s)},k-1)) + {minimum(s)}|;
+      |(set z | z in s-{minimum(s)} && z < elemth(s-{minimum(s)},k-1)) + {minimum(s)}|;
+
+    }
+  }
+}
+
+
+
+lemma {:induction s} lelemthrev(s:set<int>,x:int,k:int)
+requires 0<=k<|s| && x in s && |smaller(s,x)|==k
+ensures x==elemth(s,k)
+{
+ if (k==0){  
+   assert smaller(s,x)=={};
+   assert forall z | z in s && z!=x :: z>x;
+   lminimumrev(s,x);
+   assert x==minimum(s);
+   }
+ else{ 
+   var minim:=minimum(s);
+   if (minim==x){smallerMin(s);}
+   else{
+
+     assume |smaller(s-{minim},x)|==k-1;
+     lelemthrev(s-{minim},x,k-1);
+   }
+   }
+
+}
+
+
+lemma {:verify true} firstAndLast(s:set<int>)
+requires s!={}
+ensures minimum(s)==elemth(s,0)
+ensures maximum(s)==elemth(s,|s|-1)
+{ 
+  if (|s|==1) {
+    lMaxMinOne(s);
+    assert |s|-1==0;
+    assert maximum(s)==minimum(s)==elemth(s,0);}
+  else{
+        var minim:=minimum(s);
+        lminimum(s);
+
+      calc ==
+      { elemth(s,|s|-1);{assert |s|-1 != 0;}
+        elemth(s-{minim},|s|-2);
+         { assert s-{minim}<s;
+         assert |s-{minim}|==|s|-1;
+           firstAndLast(s-{minim});}
+        maximum(s-{minim});{max2Elems(s);}
+        maximum(s);
+      }
+  }}
